\begin{subequations}
\label{eq:linedetection-clarke}
\begin{align}
\label{eq:linedetection-clarke-1}
T(n)& = c_{1} (\tfrac{n}{2r} + 1) + c_{2} \sum_{y=0}^{\tfrac{n}{2r}}
 \left(\tfrac{n}{2r} + 1\right) + c_3 \sum_{y=0}^{\tfrac{n}{2r}}
 \sum_{x=0}^{\tfrac{n}{2r}} r^2 + c_4 \sum_{y=0}^{\tfrac{n}{2r}}
 \sum_{x=0}^{\tfrac{n}{2r}} \tfrac{1}{25}(r^2 - 2)^2 \\
& \quad + (c_{5} + c_{6} + c_{7}) \sum_{y=0}^{\tfrac{n}{2r}} \sum_{x=0}^{\tfrac{n}{2r}} 1
+ c_8 \sum_{y=0}^{\tfrac{n}{2r}} 1 \nonumber \\
\label{eq:linedetection-clarke-2}
T(n)& = (c_{1} + c_{8}) (\tfrac{n}{2r} + 1) + c_{3} r^2 (\tfrac{n}{2r} + 1)^2
+ c_{4} \tfrac{1}{25} (r^2 - 2)^2 (\tfrac{n}{2r} + 1)^2 \\
& \quad + (c_{2} + c_{5} + c_{6} + c_{7}) (\tfrac{n}{2r} + 1)^2 \nonumber \\
\label{eq:linedetection-clarke-2}
T(n)& = r^2(\tfrac{n}{2r} + 1)^2 + (r^2 - 2)^2 (\tfrac{n}{2r} + 1)^2 + (\tfrac{n}{2r} + 1)^2 + \tfrac{n}{2r} + 1
\end{align}
\end{subequations}
